add disproof of lemma 2.5

SSL.thy
@@ -37,6 +37,8 @@ datatype form =
 | Neg form          ("\<not>\<^sub>s _")
 
 abbreviation t :: form where "t \<equiv> Emp \<or>\<^sub>s \<not>\<^sub>sEmp"
+abbreviation magic_wand :: "form \<Rightarrow> form \<Rightarrow> form" (infix "-\<^emph>" 60) where 
+  "magic_wand P Q \<equiv> \<not>\<^sub>s(P-\<otimes>\<not>\<^sub>sQ)"
 
 fun size :: "form \<Rightarrow> nat" where
   "size Emp = 1"
@@ -104,6 +106,11 @@ definition weak_heap_union :: "heap \<Rightarrow> heap \<Rightarrow> heap option
 lemma weak_heap_union_sym: "(((h1::heap) ++ h2)::heap option) = (h2 ++ h1)"
   unfolding weak_heap_union_def by (auto simp: map_add_comm)
 
+lemma weak_heap_unionE: "h1 ++ h2 = Some h \<Longrightarrow> (dom h1 \<inter> dom h2 = {}) \<and> h=h1++h2"
+  apply (auto simp: weak_heap_union_def)
+  apply (metis disjoint_iff insertI1 insert_dom option.distinct(1))
+  by (metis option.discI option.inject)
+
 text \<open>Strong heap union\<close>
 definition heap_union :: "heap \<Rightarrow> stack \<Rightarrow> heap \<Rightarrow> heap option" ("_ \<uplus>\<^sup>_ _") where
   "h1 \<uplus>\<^sup>s h2 = (if (dom h1 \<inter> ran h2) \<union> (dom h2 \<inter> ran h1) \<subseteq> ran s then h1 ++ h2 else None)"
@@ -111,7 +118,14 @@ definition heap_union :: "heap \<Rightarrow> stack \<Rightarrow> heap \<Rightarr
 lemma heap_union_sym: "h1 \<uplus>\<^sup>s h2 = h2 \<uplus>\<^sup>s h1"
   unfolding heap_union_def by (auto simp: weak_heap_union_sym)
 lemma heap_union_sym_impl: "x = h1 \<uplus>\<^sup>s h2 \<Longrightarrow> x = h2 \<uplus>\<^sup>s h1"
-  by (auto simp: heap_union_sym)  
+  by (auto simp: heap_union_sym)
+lemma heap_unionE: "h1 \<uplus>\<^sup>s h2 = Some h \<Longrightarrow> ((dom h1 \<inter> ran h2) \<union> (dom h2 \<inter> ran h1) \<subseteq> ran s) \<and>
+  (dom h1 \<inter> dom h2 = {}) \<and> h=h1++h2"
+  apply (auto simp: heap_union_def weak_heap_unionE)
+  apply (meson IntI domI in_mono option.distinct(1))
+  apply (meson IntI domI in_mono option.distinct(1))
+  apply (metis disjoint_iff domIff option.distinct(1) weak_heap_union_def)
+  by (metis option.inject option.simps(3) weak_heap_union_def)
   
 lemma heap_union_model: "\<lbrakk>heap m = h; stack m = s; Some h = h1 \<uplus>\<^sup>s h2\<rbrakk> \<Longrightarrow> (s,h1) \<in> 
   {(s::stack,h::heap) |s h. finite (dom s) \<and> finite (dom h) \<and> (\<exists>l. s Nil = Some l \<and> l \<notin> dom h)}"
@@ -127,10 +141,10 @@ lemma heap_union_model':
   by (metis UnE domIff dom_map_add option.distinct(1) option.inject snd_eqD weak_heap_union_def)
   
 subsection \<open>Semantics\<close>
-fun list_segment :: "heap \<Rightarrow> loc \<Rightarrow> loc \<Rightarrow> nat \<Rightarrow> bool" where
-  "list_segment _ _ _ 0 = False"
-| "list_segment h l1 l2 (Suc 0) = (h = [l1\<mapsto>l2])"
-| "list_segment h l1 l2 (Suc n) = (\<exists>h' l1'. h=h'++[l1\<mapsto>l1'] \<and> l1 \<notin> dom h' \<and> list_segment h' l1' l2 n)"
+fun list_segment :: "nat \<Rightarrow> heap \<Rightarrow> loc \<Rightarrow> loc \<Rightarrow> bool" where
+  "list_segment 0 _ _ _ = False"
+| "list_segment (Suc 0) h l1 l2 = (h = [l1\<mapsto>l2])"
+| "list_segment (Suc n) h l1 l2 = (\<exists>h' l1'. h=h'++[l1\<mapsto>l1'] \<and> list_segment n h' l1' l2)"
 
 fun satisfies :: "(stack\<times>heap) \<Rightarrow> form \<Rightarrow> bool" where
   "satisfies (s,h) Emp = (dom h = {})"
@@ -138,7 +152,7 @@ fun satisfies :: "(stack\<times>heap) \<Rightarrow> form \<Rightarrow> bool" whe
 | "satisfies (s,h) (x\<noteq>\<^sub>sy) = (dom h = {} \<and> (\<exists>x' y'. s x = Some x' \<and> s y = Some y' \<and> x'\<noteq>y'))"
 | "satisfies (s,h) (x\<mapsto>\<^sub>sy) = (\<exists>x' y'. s x = Some x' \<and> s y = Some y' \<and> h = [x'\<mapsto>y'])"
 | "satisfies (s,h) (ls (x,y)) = (\<exists>lx ly. s x = Some lx \<and> s y = Some ly \<and> 
-    ((dom h = {} \<and> lx=ly) \<or> (\<exists>n. list_segment h lx ly n)))"
+    ((dom h = {} \<and> lx=ly) \<or> (\<exists>n. list_segment n h lx ly)))"
 | "satisfies (s,h) (\<phi>1 \<and>\<^sub>s \<phi>2) = (satisfies (s,h) \<phi>1 \<and> satisfies (s,h) \<phi>2)"
 | "satisfies (s,h) (\<phi>1 \<or>\<^sub>s \<phi>2) = (satisfies (s,h) \<phi>1 \<or> satisfies (s,h) \<phi>2)"
 | "satisfies (s,h) (\<not>\<^sub>s \<phi>) = Not (satisfies (s,h) \<phi>)"
@@ -165,5 +179,169 @@ lift_definition weak_satisfies_model :: "model \<Rightarrow> form \<Rightarrow> 
 lemma weak_strong_atoms: "atom P \<Longrightarrow> satisfies (s,h) P \<longleftrightarrow> weak_satisfies (s,h) P"
   by (induction P) auto
 lemma weak_strong_watom_model: "atom P \<Longrightarrow> m \<Turnstile> P \<longleftrightarrow> m \<Turnstile>\<^sub>w P"
-  apply transfer' using weak_strong_atoms by fast  
+  apply transfer' using weak_strong_atoms by fast
+
+definition ssl_sat :: "var set \<Rightarrow> form \<Rightarrow> bool" where
+  "ssl_sat x \<phi> \<equiv> \<exists>s h. x=dom s \<and> satisfies (s,h) \<phi>"
+definition ssl_entails :: "form \<Rightarrow> var set \<Rightarrow> form \<Rightarrow> bool" ("_ \<turnstile>\<^sub>_ _") where
+  "\<phi> \<turnstile>\<^sub>x \<psi> \<equiv> \<forall>s h. x=dom s \<and> satisfies (s,h) \<phi> \<longrightarrow> satisfies (s,h) \<psi>"
+
+fun positive :: "form \<Rightarrow> bool" where
+  "positive (P \<^emph> Q) = (positive P \<and> positive Q)"
+| "positive (P -\<otimes> Q) = (positive P \<and> positive Q)"
+| "positive (P\<and>\<^sub>sQ) = (positive P \<and> positive Q)"
+| "positive (P\<or>\<^sub>sQ) = (positive P \<and> positive Q)"
+| "positive (\<not>\<^sub>s _) = False"
+| "positive _ = True"
+
+subsection \<open>Disproof of stronger statement of lemma 2.5\<close>
+lemma counter1: "
+  weak_satisfies ([Var 0 \<mapsto> 0, Var 2 \<mapsto> 2, Nil \<mapsto> 3], [0\<mapsto>1,1\<mapsto>2,2\<mapsto>1]) (LS (Var 0,Var 2))"
+  (is "weak_satisfies (?s,?h) _")
+proof -
+  have "list_segment 1 [1\<mapsto>2] 1 2" by simp
+  moreover have "[1::nat\<mapsto>2::nat,2\<mapsto>1] = [1\<mapsto>2]++[2\<mapsto>1]" by auto
+  ultimately have "\<exists>h' l1'. [1\<mapsto>2,2\<mapsto>1]=h'++[2\<mapsto>l1'] \<and> list_segment 1 h' l1' 2" by auto
+  then have "list_segment (Suc 1) [1\<mapsto>2,2\<mapsto>1] 2 2" by simp
+  moreover have "[1::nat\<mapsto>2::nat,2\<mapsto>1] = [1\<mapsto>2,2\<mapsto>1]++[1\<mapsto>2]" by auto
+  ultimately have "\<exists>h' l1'. [1\<mapsto>2,2\<mapsto>1]=h'++[1\<mapsto>l1'] \<and> list_segment (Suc 1) h' l1' 2" by blast
+  then have "list_segment (Suc (Suc 1)) [1\<mapsto>2,2\<mapsto>1] 1 2" by simp
+  moreover have "[0::nat\<mapsto>1::nat,1\<mapsto>2,2\<mapsto>1] = [1\<mapsto>2,2\<mapsto>1]++[0\<mapsto>1]" by auto
+  ultimately have "\<exists>h' l1'. ?h=h'++[0\<mapsto>l1'] \<and> list_segment (Suc (Suc 1)) h' l1' 2" by blast
+  then have "list_segment (Suc (Suc (Suc 1))) ?h 0 2" by simp
+  then have "?s (Var 0) = Some 0 \<and> ?s (Var 2) = Some 2 \<and> ((dom ?h = {} \<and> 0=2) \<or> (\<exists>n. list_segment n ?h 0 2))"
+    by fastforce
+  then have "\<exists>l0 l2. ?s (Var 0) = Some l0 \<and> ?s (Var 2) = Some l2 \<and> ((dom ?h = {} \<and> l0=l2) 
+    \<or> (\<exists>n. list_segment n ?h l0 l2))" by simp
+  then show ?thesis by simp
+qed
+lemma counter2: "positive (LS (Var 0,Var 2))" by simp
+lemma counter3: "{l. [0::nat\<mapsto>1::nat,1\<mapsto>2,2\<mapsto>1] l = Some 1} = {0,2} \<and> 1 \<notin> ran [Var 0 \<mapsto> 0::nat, Var 2 \<mapsto> 2, Nil \<mapsto> 3]"
+  by auto
+
+lemma disproof: "\<not>(\<forall>\<phi> s h. (positive \<phi> \<longrightarrow>weak_satisfies (s,h) \<phi> \<longrightarrow>
+  (ran h - dom h \<subseteq> ran s) \<and> (\<forall>l. (\<exists>x y. x\<noteq>y \<and> h x = Some l \<and> h y = Some l) \<longrightarrow> l \<in> ran s) \<and>
+  (dom h - ran h \<subseteq> ran s)))" (is "\<not>?P")
+proof
+  define h::heap where "h=[0 \<mapsto> 1, 1 \<mapsto> 2, 2 \<mapsto> 1]" 
+  define s::stack where "s=[Var 0 \<mapsto> 0, Var 2 \<mapsto> 2, var.Nil \<mapsto> 3]"
+  assume ?P
+  then have "positive \<phi> \<Longrightarrow> weak_satisfies (s,h) \<phi> \<Longrightarrow>
+    (ran h - dom h \<subseteq> ran s) \<and> (\<forall>l. (\<exists>x y. x\<noteq>y \<and> h x = Some l \<and> h y = Some l) \<longrightarrow> l \<in> ran s) \<and>
+    (dom h - ran h \<subseteq> ran s)" for \<phi> s h by simp
+  from this[OF counter2 counter1] have "(\<forall>l. (\<exists>x y. x \<noteq> y \<and> h x = Some l \<and> h y = Some l) \<longrightarrow> l \<in> ran s)" 
+    by (auto simp: h_def s_def)
+  then have "1 \<in> ran s" unfolding h_def by auto (metis fun_upd_other fun_upd_same nat.distinct(1) numeral_2_eq_2)
+  with counter3 s_def show False by simp
+qed
+    
+
+lemma 
+assumes "positive \<phi>" "weak_satisfies (s,h) \<phi>"
+shows "(ran h - dom h \<subseteq> ran s) \<and> (\<forall>l. (\<exists>x y. x\<noteq>y \<and> h x = Some l \<and> h y = Some l) \<longrightarrow> l \<in> ran s) \<and>
+  (dom h - ran h \<subseteq> ran s)"
+using assms proof (induction \<phi> arbitrary: s h)
+case Emp
+  then have "h=Map.empty" by auto
+  then have "ran h = {}" "dom h = {}" "\<forall>x. h x = None" by auto
+  then show ?case by auto
+next
+  case (PointsTo x1 x2)
+  then obtain y1 y2 where s: "s x1 = Some y1" "s x2 = Some y2" by auto
+  with PointsTo have "h=[y1\<mapsto>y2]" by simp
+  with s show ?case apply auto
+    apply (smt (verit, ccfv_SIG) mem_Collect_eq option.simps(3) ran_def)
+    by (metis option.discI ranI)
+next
+  case (LS x)
+  obtain x1 x2 where "x=(x1,x2)" by fastforce
+  with LS(2) obtain y1 y2 where "s x1 = Some y1" "s x2 = Some y2" 
+    "((dom h = {} \<and> y1=y2) \<or> (\<exists>n. n list_segment h y1 y2))" by fastforce
+  then show ?case sorry
+next
+  case (Eq x1 x2)
+  then have "h=Map.empty" by auto
+  then have "ran h = {}" "dom h = {}" "\<forall>x. h x = None" by auto
+  then show ?case by auto
+next
+  case (NEq x1 x2)
+  then have "h=Map.empty" by auto
+  then have "ran h = {}" "dom h = {}" "\<forall>x. h x = None" by auto
+  then show ?case by auto
+next
+  case (SepConj \<phi>1 \<phi>2)
+  then obtain h1 h2 where h12: "h1 ++ h2 = Some h" "weak_satisfies (s,h1) \<phi>1" "weak_satisfies (s,h2) \<phi>2"
+    by auto
+  from SepConj(3) have pos: "positive \<phi>1" "positive \<phi>2" by simp_all
+  from weak_heap_unionE[OF h12(1)] have "dom h1 \<inter> dom h2 = {}" "dom h = dom h1 \<union> dom h2" "ran h = ran h1 \<union> ran h2"
+    by (auto simp: weak_heap_union_def ran_map_add)
+  with SepConj(1)[OF pos(1) h12(2)] SepConj(2)[OF pos(2) h12(3)] show ?case apply auto
+    by (smt (verit) Diff_iff \<open>dom h1 \<inter> dom h2 = {} \<and> h = h1 ++ h2\<close> disjoint_iff in_mono map_add_Some_iff ranI)  
+next
+  case (Septraction \<phi>1 \<phi>2)
+  then obtain h0 h1 where h01: "Some h1 = h0++h" "weak_satisfies (s,h0) \<phi>1" "weak_satisfies (s,h1) \<phi>2"
+    by auto (metis weak_heap_union_sym)
+  from Septraction(3) have pos: "positive \<phi>1" "positive \<phi>2" by simp_all
+  from weak_heap_unionE[OF h01(1)[symmetric]] have dom_ran: "dom h0 \<inter> dom h = {}" "dom h1 = dom h0 \<union> dom h"
+    "ran h1 = ran h \<union> ran h0" by (auto simp: ran_map_add)
+  then have join: "(\<exists>x y. x\<noteq>y \<and> h x = Some l \<and> h y = Some l) \<longrightarrow> (\<exists>x y. x\<noteq>y \<and> h1 x = Some l \<and> h1 y = Some l)" for l
+    by auto (metis \<open>dom h0 \<inter> dom h = {} \<and> h1 = h0 ++ h\<close> map_add_find_right)
+  \<comment> \<open>For a dangling pointer l in h, it is either also dangling in h1 or a join point in h1 
+    or pointing to a source in h0.\<close>
+  from dom_ran have "(h l = Some l' \<and> l' \<in> ran h - dom h) \<Longrightarrow> (l' \<in> ran h1 - dom h1 \<or> 
+    (\<exists>x y. x\<noteq>y \<and> h1 x = Some l' \<and> h1 y = Some l') \<or> l' \<in> dom h0 - ran h0)" for l l'
+    by auto (smt (verit, ccfv_threshold) \<open>dom h0 \<inter> dom h = {} \<and> h1 = h0 ++ h\<close> disjoint_iff domI 
+      map_add_dom_app_simps(1) map_add_dom_app_simps(3) mem_Collect_eq ran_def)
+  with Septraction(1)[OF pos(1) h01(2)] Septraction(2)[OF pos(2) h01(3)] join
+  show ?case apply auto apply (smt (verit, ccfv_threshold) DiffI domD in_mono mem_Collect_eq ran_def)
+  by (metis DiffI Un_iff \<open>dom h0 \<inter> dom h = {} \<and> h1 = h0 ++ h\<close> disjoint_iff domIff dom_map_add dom_ran(3) in_mono inf_sup_aci(5) option.distinct(1))
+next
+  case (Conj \<phi>1 \<phi>2)
+  then have "weak_satisfies (s,h) \<phi>1" "weak_satisfies (s,h) \<phi>2" by auto
+  from Conj(1)[OF _ this(1)] Conj(2)[OF _ this(2)] Conj(3) show ?case by auto
+next
+  case (Disj \<phi>1 \<phi>2)
+  then have sat: "weak_satisfies (s,h) \<phi>1 \<or> weak_satisfies (s,h) \<phi>2" by auto
+  from Disj(3) have "positive \<phi>1" "positive \<phi>2" by auto
+  with sat Disj(1,2) show ?case by auto blast+
+next
+  case (Neg \<phi>)
+  then show ?case by simp
+qed
+
+(* lemma "list_segment n h l1 l2 \<Longrightarrow> l1 \<in> dom h \<and> l2 \<in> ran h \<and> 
+    (\<forall>l. (\<exists>x y. x\<noteq>y \<and> h x = Some l \<and> h y = Some l) \<longrightarrow> l=l2)
+    \<and> ran h - dom h \<subseteq> {l2} \<and> dom h - ran h \<subseteq> {l1}"
+proof (induction n h l1 l2 rule: list_segment.induct)
+  case (1 uu uv uw)
+  then show ?case by simp
+next
+  case (2 h l1 l2)
+  then have "h = [l1\<mapsto>l2]" by simp
+  then show ?case by (auto simp: ran_def)
+next
+  case (3 v h l1 l2)
+  then obtain h' l1' where h': "h=h'++[l1\<mapsto>l1']" "l1 \<notin> dom h'" "list_segment (Suc v) h' l1' l2" 
+    by auto
+  from h'(1,2) have dom_ran: "dom h = dom h' \<union> {l1}" "ran h = ran h' \<union> {l1'}" by auto
+  from dom_ran 3(1)[OF h'(3)] have "l1 \<in> dom h" "l2 \<in> ran h" by auto
+  moreover from dom_ran 3(1)[OF h'(3)] have "ran h - dom h \<subseteq> {l2}" by auto
+  moreover from dom_ran 3(1)[OF h'(3)] have "dom h - ran h \<subseteq> {l1}" by auto
+  moreover {
+    fix l
+    assume "(\<exists>x y. x \<noteq> y \<and> h x = Some l \<and> h y = Some l)"
+    then obtain x y where xy: "x \<noteq> y \<and> h x = Some l \<and> h y = Some l" by auto
+    with 3(1)[OF h'(3)] h'(1,2) have "x \<in> dom h' \<and> y \<in> dom h' \<Longrightarrow> h' x = Some l \<and> h' y = Some l" 
+      apply auto apply (metis option.distinct(1)) by (metis is_none_code(2) is_none_simps(1))
+    with 3(1)[OF h'(3)] xy have "x \<in> dom h' \<and> y \<in> dom h' \<Longrightarrow> l = l2" by auto
+    from xy 3(1)[OF h'(3)] h'(1,2) have "\<not>(x \<in> dom h' \<and> y \<in> dom h') \<Longrightarrow> l = l1'"
+      by auto (metis option.inject)+
+    moreover from xy h'(1) have "\<not>(x \<in> dom h' \<and> y \<in> dom h') \<Longrightarrow> x\<in>dom h' \<or>y\<in>dom h'" 
+      apply auto apply (metis option.distinct(1)) by (metis option.distinct(1))
+    ultimately have "\<not>(x \<in> dom h' \<and> y \<in> dom h') \<Longrightarrow> l1' \<in> ran h'" using xy h'(1) apply auto
+      apply (smt (verit, best)  map_add_empty map_add_upd map_upd_Some_unfold ranI) by (metis ranI)
+  }
+  ultimately show ?case apply auto
+qed *)
+
 end
