ROOT
@@ -1,5 +1,5 @@
 session ssl = "HOL-Library" +
-  options [document = pdf, document_output = "output"]
+  options [document = pdf, document_output = "output", quick_and_dirty]
   theories [document = false]
     SSL
     ModelIso
